compiler/backend/stackLangScript.sml
@@ -21,8 +21,9 @@ val _ = Datatype `
        | FFI num num num num (* FFI index, array_ptr, array_len, ret_addr *)
        | Tick
        (* new in stackLang, compared to wordLang, below *)
-       | StackAlloc num
-       | StackFree num
+       | LocValue num num num   (* assign v1 := Loc v2 v3 *)
+       | StackAlloc num         (* allocate n slots on the stack *)
+       | StackFree num          (* free n slots on the stack *)
        | StackStore num num     (* offset, fast *)
        | StackStoreAny num num  (* reg contains offset, slow, used by GC *)
        | StackLoad num num      (* offset, fast *)
